src/ReactorModel/Components/Lift.lean
@@ -35,18 +35,17 @@ def fromRaw
   {rcn : Raw.Reaction} (hr : ∃ i, rtr.rcns i = rcn) 
   {raw : Raw.Change} {i} (hc : raw ∈ rcn.body i) : 
   Change :=
-  match hm:raw with 
+  match raw with 
     | Raw.Change.port target value        => Change.port target value  
     | Raw.Change.state target value       => Change.state target value 
     | Raw.Change.action target time value => Change.action target time value 
     | Raw.Change.connect src dst          => Change.connect src dst    
     | Raw.Change.disconnect src dst       => Change.disconnect src dst 
     | Raw.Change.delete rtrID             => Change.delete rtrID
-    | Raw.Change.create cr id => 
-      Change.create (id := id) $ Reactor.fromRaw cr (by
-          have ha := Raw.Reactor.Ancestor.creatable hr.choose_spec hc
-          exact Raw.Reactor.Ancestor.preserves_wf ha hw
-      )
+    | Raw.Change.create cr => 
+      let ha := Raw.Reactor.Ancestor.creatable hr.choose_spec hc
+      let hw' := Raw.Reactor.Ancestor.preserves_wf ha hw
+      Change.create (Reactor.fromRaw cr hw')
 
 -- To ensure that `Change.fromRaw` performs a sensible transformation from
 -- raw to "proper" changes, we define what it means for raw and "proper"
@@ -54,18 +53,18 @@ def fromRaw
 -- This notion of equivalence is then used in `Change.fromRaw_rawEquiv` to
 -- prove that `Change.fromRaw` produces only equivalent changes.
 inductive RawEquiv : Change → Raw.Change → Prop
-  | port       {t v} :                              RawEquiv (Change.port t v) (Raw.Change.port t v)
-  | state      {t v} :                              RawEquiv (Change.state t v) (Raw.Change.state t v)
-  | action     {t tm v} :                           RawEquiv (Change.action t tm v) (Raw.Change.action t tm v)
-  | connect    {s d} :                              RawEquiv (Change.connect s d) (Raw.Change.connect s d)
-  | disconnect {s d} :                              RawEquiv (Change.disconnect s d) (Raw.Change.disconnect s d)
-  | create     {r r' i} : (Reactor.RawEquiv r r') → RawEquiv (Change.create r i) (Raw.Change.create r' i)
-  | delete     {i} :                                RawEquiv (Change.delete i) (Raw.Change.delete i)
+  | port       {t v} :                            RawEquiv (Change.port t v) (Raw.Change.port t v)
+  | state      {t v} :                            RawEquiv (Change.state t v) (Raw.Change.state t v)
+  | action     {t tm v} :                         RawEquiv (Change.action t tm v) (Raw.Change.action t tm v)
+  | connect    {s d} :                            RawEquiv (Change.connect s d) (Raw.Change.connect s d)
+  | disconnect {s d} :                            RawEquiv (Change.disconnect s d) (Raw.Change.disconnect s d)
+  | create     {r r'} : (Reactor.RawEquiv r r') → RawEquiv (Change.create r) (Raw.Change.create r')
+  | delete     {i} :                              RawEquiv (Change.delete i) (Raw.Change.delete i)
 
 theorem RawEquiv.unique {c : Change} {raw₁ raw₂ : Raw.Change} (h₁ : RawEquiv c raw₁) (h₂ : RawEquiv c raw₂) : 
   raw₁ = raw₂ := by
   cases h₁ <;> cases h₂
-  case create.create rtr r₁ _ he r₂ he' => simp only [Reactor.RawEquiv.unique he he']
+  case create.create rtr r₁ he r₂ he' => simp only [Reactor.RawEquiv.unique he he']
   all_goals { rfl }
 
 theorem RawEquiv.fromRaw {raw : Raw.Change} {rtr rcn i} (hw hr hc) :
@@ -92,7 +91,7 @@ def fromRaw {rtr : Raw.Reactor} (hw : rtr.wellFormed) {raw : Raw.Reaction} (hr :
   children := raw.children,
   body := λ i => (raw.body i).attach.map (Change.fromRaw hw hr ·.property),
   tsSubInDeps := (hw.direct.rcnsWF hr).tsSubInDeps,
-  prtOutDepOnly := by
+  prtOutDepOnly := by 
     intro i _ v ho hc
     simp [List.mem_map] at hc
     have := (hw.direct.rcnsWF hr).prtOutDepOnly i v ho
@@ -118,7 +117,7 @@ def fromRaw {rtr : Raw.Reactor} (hw : rtr.wellFormed) {raw : Raw.Reaction} (hr :
     rw [←ha] at he
     cases he
     exact (hw.direct.rcnsWF hr).actNotPast i a t v hc,
-  normNoChild := by
+  normNoChild := by 
     intro ha
     have hn := (hw.direct.rcnsWF hr).normNoChild
     simp at ha
@@ -170,28 +169,36 @@ theorem RawEquiv.unique {rcn : Reaction} {raw₁ raw₂ : Raw.Reaction} (h₁ : 
       case cons hd₂ tl₂ hhd₂ htl₂ =>
         simp [Change.RawEquiv.unique hhd₁ hhd₂, hi tl₁ htl₁ tl₂ htl₂]
 
-/-
-https://leanprover.zulipchat.com/#narrow/stream/270676-lean4/topic/tactic.20'generalize'.20failed
-private theorem RawEquiv.fromRaw_body_aux {raw : Raw.Reaction} {rtr : Raw.Reactor} (hw : rtr.wellFormed) (rcs : List Raw.Change) :
-  ∀ raw i (hr : ∃ i, rtr.rcns i = some raw), rcs = raw.body i → List.forall₂ Change.RawEquiv ((Reaction.fromRaw hw hr).body i) (raw.body i) := by
-  simp only [Reaction.fromRaw]
-  induction rcs
-  case nil =>
-    intro raw i hr he
-    simp only [←he]
-    sorry
-  case cons =>
-    intro raw i hr he
-    simp only [←he]
--/
-
 theorem RawEquiv.fromRaw {raw : Raw.Reaction} {rtr} (hw hr) :
   RawEquiv (@Reaction.fromRaw rtr hw raw hr) raw := {
     deps := by simp [Reaction.fromRaw],
     triggers := by simp [Reaction.fromRaw],
     prio := by simp [Reaction.fromRaw],
     children := by simp [Reaction.fromRaw],
-    body := sorry
+    body := by
+      intro i
+      simp [Reaction.fromRaw]
+      generalize hl : (raw.body i).attach.map (Change.fromRaw hw hr ·.property) = l
+      generalize hl' : raw.body i = l'
+      induction l
+      case nil =>
+        simp only [←hl', List.map_eq_nil.mp hl |> (List.attach_eq_nil _).mp]
+        exact List.forall₂.nil
+      case cons hd tl hi =>
+        sorry
+        /-
+        cases hc : List.attach (raw.body p s)
+        case nil =>
+          rw [hc, List.map_nil] at h
+          contradiction
+        case cons hd' tl' =>
+          simp [hc] at h
+          cases hc' : raw.body p s
+          case nil =>
+            simp [hc'] at hc
+            sorry
+          sorry
+        -/
   }
 
 theorem RawEquiv.fromRaw' {rcn : Reaction} {rtr raw hw hr} :
