src/ReactorModel/Execution/Context.lean
@@ -2,18 +2,22 @@ import ReactorModel.Components
 
 structure Execution.Context where
   executedRcns : Time.Tag ▸ Finset ID
-  nonempty : executedRcns.nonempty
+  execedNonempty : executedRcns.nonempty
+  freshID : Reactor → ID   
+  freshIDCorrect : ∀ σ cmp, freshID σ ∉ σ.ids cmp
 
 namespace Execution.Context
 
 -- An extensionality theorem for `Context`.
-theorem ext_iff {ctx₁ ctx₂ : Context} : ctx₁ = ctx₂ ↔ ctx₁.executedRcns = ctx₂.executedRcns := by
+theorem ext_iff {ctx₁ ctx₂ : Context} : 
+  ctx₁ = ctx₂ ↔ 
+  ctx₁.executedRcns = ctx₂.executedRcns ∧ ctx₁.freshID = ctx₂.freshID := by
   constructor
   case mp => intro h; simp [h]
   case mpr => intro h; cases ctx₁; cases ctx₂; simp [h]
 
 def time (ctx : Context) : Time.Tag :=
-  ctx.executedRcns.ids.max' ⟨ctx.nonempty.choose, Finmap.ids_def.mpr ctx.nonempty.choose_spec⟩
+  ctx.executedRcns.ids.max' ⟨ctx.execedNonempty.choose, Finmap.ids_def.mpr ctx.execedNonempty.choose_spec⟩
 
 theorem executedRcns_at_time_isSome (ctx : Context) :
   (ctx.executedRcns ctx.time).isSome := by
@@ -31,7 +35,9 @@ theorem currentExecutedRcns_def (ctx : Context) : some ctx.currentExecutedRcns =
 
 noncomputable def addCurrentExecuted (ctx : Context) (i : ID) : Context := {
   executedRcns := ctx.executedRcns.update ctx.time $ ctx.currentExecutedRcns.insert i,
-  nonempty := ctx.executedRcns.update_nonempty _ _ ctx.nonempty
+  execedNonempty := ctx.executedRcns.update_nonempty _ _ ctx.execedNonempty,
+  freshID := ctx.freshID,
+  freshIDCorrect := ctx.freshIDCorrect
 }
 
 theorem addCurrentExecuted_same_time (ctx : Context) (i : ID) : (ctx.addCurrentExecuted i).time = ctx.time := by 
@@ -42,7 +48,9 @@ theorem addCurrentExecuted_same_time (ctx : Context) (i : ID) : (ctx.addCurrentE
 
 noncomputable def advanceTime (ctx : Context) (g : Time.Tag) (h : ctx.time < g) : Context := {
   executedRcns := ctx.executedRcns.update' g ∅,
-  nonempty := ctx.executedRcns.update_nonempty _ _ ctx.nonempty
+  execedNonempty := ctx.executedRcns.update_nonempty _ _ ctx.execedNonempty,
+  freshID := ctx.freshID,
+  freshIDCorrect := ctx.freshIDCorrect
 }
 
 theorem advanceTime_strictly_increasing (ctx : Context) (g : Time.Tag) (h : ctx.time < g) :
